Move some theorems around; mainly to put cfindleast into churchnumTheory.

examples/computability/lambda/churchnumScript.sml
@@ -8,6 +8,7 @@ open normal_orderTheory
 open churchboolTheory
 open churchpairTheory
 open reductionEval
+open stepsTheory
 
 fun Store_thm(n,t,tac) = store_thm(n,t,tac) before export_rewrites [n]
 
@@ -721,6 +722,201 @@ val cnsnd_behaviour = store_thm(
   ``cnsnd @@ church p -n->* church (nsnd p)``,
   SIMP_TAC (bsrw_ss()) [cnsnd_def, nsnd_def, cminus_behaviour,
                         cinvtri_behaviour, ctri_behaviour]);
+
+(* ----------------------------------------------------------------------
+    cfindleast
+   ---------------------------------------------------------------------- *)
+
+val cfindbody_def = Define`
+  cfindbody P N =
+    let lp = NEW (FV P) in
+    let nv = NEW (FV P ∪ {lp})
+    in
+        Yf (LAM lp (LAM nv (P @@ VAR nv
+                              @@ VAR nv
+                              @@ (VAR lp @@ (csuc @@ VAR nv))))) @@ N
+`;
+
+val fresh_cfindbody = store_thm(
+  "fresh_cfindbody",
+  ``lp ∉ FV P ∧ nv ≠ lp ∧ nv ∉ FV P ⇒
+    (cfindbody P N = Yf (LAM lp (LAM nv (P @@ VAR nv @@ VAR nv
+                                           @@ (VAR lp @@ (csuc @@ VAR nv))))) @@
+                        N)``,
+  SRW_TAC [][LET_THM, cfindbody_def] THEN
+  binderLib.NEW_ELIM_TAC THEN REPEAT STRIP_TAC THEN
+  binderLib.NEW_ELIM_TAC THEN REPEAT STRIP_TAC THEN
+  SRW_TAC [][termTheory.LAM_eq_thm, termTheory.tpm_fresh] THEN
+  Cases_on `nv = v` THEN SRW_TAC [][termTheory.tpm_fresh] THEN
+  Cases_on `lp = v'` THEN SRW_TAC [][termTheory.tpm_fresh] THEN
+  METIS_TAC []);
+
+val cfindbody_SUB = store_thm(
+  "cfindbody_SUB",
+  ``[Q/v] (cfindbody P N) = cfindbody ([Q/v]P) ([Q/v]N)``,
+  Q_TAC (NEW_TAC "lp") `FV P ∪ FV Q ∪ {v}` THEN
+  Q_TAC (NEW_TAC "nv") `FV P ∪ FV Q ∪ {v;lp}` THEN
+  `cfindbody P N = Yf (LAM lp (LAM nv (P @@ VAR nv @@ VAR nv
+                                         @@ (VAR lp @@ (csuc @@ VAR nv))))) @@
+                    N`
+    by SRW_TAC [][fresh_cfindbody] THEN
+  `cfindbody ([Q/v]P) ([Q/v]N) =
+   Yf (LAM lp (LAM nv ([Q/v]P @@ VAR nv @@ VAR nv
+                            @@ (VAR lp @@ (csuc @@ VAR nv))))) @@ [Q/v]N`
+    by (MATCH_MP_TAC (GEN_ALL fresh_cfindbody) THEN
+        SRW_TAC [][chap2Theory.NOT_IN_FV_SUB]) THEN
+  SRW_TAC [][termTheory.lemma14b]);
+
+val cfindbody_thm = store_thm(
+  "cfindbody_thm",
+  ``cfindbody P N -w->* P @@ N @@ N @@ cfindbody P (csuc @@ N)``,
+  unvarify_tac head_reductionTheory.whstar_substitutive THEN
+  SRW_TAC [][cfindbody_SUB, termTheory.lemma14b] THEN
+  Q_TAC (NEW_TAC "z") `{Ps}` THEN
+  Q_TAC (NEW_TAC "nv") `{Ps; z}` THEN
+  `∀N. cfindbody (VAR Ps) N =
+       Yf (LAM z (LAM nv (VAR Ps @@ VAR nv @@ VAR nv
+                              @@ (VAR z @@ (csuc @@ VAR nv)))))
+       @@ N`
+     by SRW_TAC [][fresh_cfindbody] THEN
+  ASM_SIMP_TAC (whfy (srw_ss())) [MATCH_MP relationTheory.RTC_SUBSET
+                                           head_reductionTheory.whY2]);
+
+
+val cfindbody_cong = store_thm(
+  "cfindbody_cong",
+  ``P == P' ⇒ N == N' ⇒ cfindbody P N == cfindbody P' N'``,
+  Q_TAC (NEW_TAC "lp") `FV P ∪ FV P'` THEN
+  Q_TAC (NEW_TAC "nv") `FV P ∪ FV P' ∪ {lp}` THEN
+  REPEAT STRIP_TAC THEN
+  `(cfindbody P N = Yf (LAM lp (LAM nv (P @@ VAR nv @@ VAR nv
+                                         @@ (VAR lp @@ (csuc @@ VAR nv))))) @@
+                   N) ∧
+   (cfindbody P' N' =
+      Yf (LAM lp (LAM nv (P' @@ VAR nv @@ VAR nv
+                             @@ (VAR lp @@ (csuc @@ VAR nv))))) @@
+      N')`
+    by SRW_TAC [][fresh_cfindbody] THEN
+  ASM_SIMP_TAC (bsrw_ss()) []);
+
+val bnf_cfindbody = Store_thm(
+  "bnf_cfindbody",
+  ``¬bnf (cfindbody P N)``,
+  SRW_TAC [][cfindbody_def, LET_THM]);
+
+val cfindleast_def = Define`
+  cfindleast = LAM "P" (cfindbody (VAR "P") (church 0))
+`;
+
+val FV_cfindleast = Store_thm(
+  "FV_cfindleast",
+  ``FV cfindleast = {}``,
+  SRW_TAC [][cfindleast_def, cfindbody_def, LET_THM,
+             pred_setTheory.EXTENSION] THEN METIS_TAC []);
+
+val cfindleast_termI = store_thm(
+  "cfindleast_termI",
+  ``(∀n. ∃b. P @@ church n == cB b) ∧ P @@ church n == cB T ⇒
+    cfindleast @@ P == church (LEAST n. P @@ church n == cB T)``,
+  STRIP_TAC THEN numLib.LEAST_ELIM_TAC THEN CONJ_TAC THEN1 METIS_TAC [] THEN
+  POP_ASSUM (K ALL_TAC) THEN
+  SIMP_TAC (bsrw_ss()) [cfindleast_def, cfindbody_SUB] THEN
+  Q_TAC SUFF_TAC
+    `∀p n. p ≤ n ∧
+           (∀m. m < n ⇒ ¬(P @@ church m == cB T)) ∧
+           P @@ church n == cB T ⇒
+           cfindbody P (church p) == church n`
+    THEN1 METIS_TAC [DECIDE ``0 ≤ n``] THEN
+  Induct_on `n - p` THEN REPEAT STRIP_TAC THENL [
+    `p = n` by DECIDE_TAC THEN
+    ASM_SIMP_TAC (bsrw_ss()) [Once cfindbody_thm, cB_behaviour],
+
+    `p < n` by DECIDE_TAC THEN
+    `∃r. P @@ church p == cB r` by METIS_TAC [] THEN
+    `r = F` by (Cases_on `r` THEN METIS_TAC []) THEN
+    ASM_SIMP_TAC (bsrw_ss()) [Once cfindbody_thm, cB_behaviour,
+                              csuc_behaviour, Cong cfindbody_cong] THEN
+    FIRST_X_ASSUM (fn th => MATCH_MP_TAC (REWRITE_RULE [AND_IMP_INTRO] th)) THEN
+    ASM_SIMP_TAC (srw_ss() ++ ARITH_ss) []
+  ]);
+
+val cfindbody_11 = Store_thm(
+  "cfindbody_11",
+  ``(cfindbody P1 N1 = cfindbody P2 N2) = (P1 = P2) ∧ (N1 = N2)``,
+  Q_TAC (NEW_TAC "lp") `FV P1 ∪ FV P2` THEN
+  Q_TAC (NEW_TAC "nv") `FV P1 ∪ FV P2 ∪ {lp}` THEN
+  `(cfindbody P1 N1 = Yf (LAM lp (LAM nv (P1 @@ VAR nv @@ VAR nv
+                                            @@ (VAR lp @@ (csuc @@ VAR nv)))))
+                       @@ N1) ∧
+   (cfindbody P2 N2 = Yf (LAM lp (LAM nv (P2 @@ VAR nv @@ VAR nv
+                                            @@ (VAR lp @@ (csuc @@ VAR nv)))))
+                       @@ N2)`
+      by SRW_TAC [][fresh_cfindbody] THEN
+  SRW_TAC [][]);
+
+val lameq_triangle = store_thm(
+  "lameq_triangle",
+  ``M == N ∧ M == P ∧ bnf N ∧ bnf P ⇒ (N = P)``,
+  METIS_TAC [chap3Theory.betastar_lameq_bnf, chap2Theory.lam_eq_rules,
+             chap3Theory.bnf_reduction_to_self]);
+
+val cfindleast_bnfE = store_thm(
+  "cfindleast_bnfE",
+  ``(∀n. ∃b. P @@ church n == cB b) ∧
+    cfindleast @@ P == r ∧ bnf r ⇒
+    ∃m. (r = church m) ∧ P @@ r == cB T ∧
+        ∀m₀. m₀ < m ⇒ P @@ church m₀ == cB F``,
+  SIMP_TAC (bsrw_ss()) [cfindleast_def, cfindbody_SUB] THEN
+  REPEAT STRIP_TAC THEN
+  `∃N. steps N (cfindbody P (church 0)) = r`
+    by METIS_TAC [nstar_steps, nstar_betastar_bnf,
+                  chap3Theory.betastar_lameq_bnf] THEN
+  Q_TAC SUFF_TAC
+    `∀N cn ct. (steps N (cfindbody P ct) = r) ⇒
+               (∀c0. c0 < cn ⇒ P @@ church c0 == cB F) ⇒
+               (ct == church cn) ⇒
+               ∃m. (r = church m) ∧ P @@ r == cB T ∧
+                   ∀m₀. m₀ < m ⇒ P @@ church m₀ == cB F`
+    THEN1 METIS_TAC [DECIDE ``¬(x < 0)``, chap2Theory.lameq_refl] THEN
+  REPEAT (FIRST_X_ASSUM (fn th => if free_in ``cfindbody`` (concl th) then
+                                    ALL_TAC
+                                  else NO_TAC)) THEN
+  completeInduct_on `N` THEN
+  MAP_EVERY Q.X_GEN_TAC [`cn`,`ct`] THEN REPEAT STRIP_TAC THEN
+  `cfindbody P ct -n->* P @@ ct @@ ct @@ (cfindbody P (csuc @@ ct))`
+     by METIS_TAC [cfindbody_thm, whstar_nstar] THEN
+  `∃b. P @@ church cn == cB b` by METIS_TAC [] THEN
+  Cases_on `b` THENL [
+    `cfindbody P ct == church cn`
+      by ASM_SIMP_TAC (bsrw_ss()) [cB_behaviour] THEN
+    `cfindbody P ct -n->* r` by METIS_TAC [steps_nstar] THEN
+    `church cn = r` by METIS_TAC [lameq_triangle, bnf_church,
+                                  nstar_betastar,
+                                  chap3Theory.betastar_lameq_bnf] THEN
+    SRW_TAC [][],
+
+    `P @@ ct == cB F` by ASM_SIMP_TAC (bsrw_ss()) [] THEN
+    POP_ASSUM (STRIP_ASSUME_TAC o
+               MATCH_MP (GEN_ALL (CONJUNCT2 whead_tests))) THEN
+    `cfindbody P ct -n->* cfindbody P (csuc @@ ct)`
+      by METIS_TAC [whstar_nstar, relationTheory.RTC_CASES_RTC_TWICE] THEN
+    `∃n1. cfindbody P (csuc @@ ct) = steps n1 (cfindbody P ct)`
+      by METIS_TAC [nstar_steps] THEN
+    `¬bnf (cfindbody P (csuc @@ ct))` by SRW_TAC [][] THEN
+    `n1 < N` by METIS_TAC [DECIDE ``n:num < m ∨ (n = m) ∨ m < n``,
+                           bnf_steps_upwards_closed] THEN
+    `∃rest. N = rest + n1` by (Q.EXISTS_TAC `N - n1` THEN DECIDE_TAC) THEN
+    FULL_SIMP_TAC (srw_ss()) [steps_plus] THEN
+    `n1 ≠ 0` by (STRIP_TAC THEN
+                 FULL_SIMP_TAC (srw_ss()) [termTheory.APP_acyclic]) THEN
+    `rest < rest + n1` by DECIDE_TAC THEN
+    POP_ASSUM (fn th1 => FIRST_X_ASSUM (MP_TAC o C MATCH_MP th1)) THEN
+    DISCH_THEN (Q.SPECL_THEN [`SUC cn`, `csuc @@ ct`] MP_TAC) THEN
+    ASM_SIMP_TAC (bsrw_ss()) [csuc_behaviour] THEN
+    DISCH_THEN MATCH_MP_TAC THEN
+    REPEAT STRIP_TAC THEN
+    `(c0 = cn) ∨ c0 < cn` by DECIDE_TAC THEN SRW_TAC [][]
+  ]);
 
 val _ = export_theory()
 
